created a seal library variant that now implements unforgeable keys (interval is now applied to this new version, but since interval does not depend on the unforgeability of keys it is provable in both versions)

theories/examples/macros_new.v
@@ -371,6 +371,195 @@ Section macros.
     iSplitL. iNext. eauto. eauto.
   Qed.
 
+  (* -------------------------------------- REQPERM ----------------------------------- *)
+  (* the following macro requires that a given registers contains a capability with a
+     given (encoded) permission. If this is not the case, the macro goes to fail,
+     otherwise it continues *)
+
+  (* TODO: move this to the rules_Get.v file. small issue with the spec of failure: it does not actually
+     require/leave a trace on dst! It would be good if req_regs of a failing get does not include dst (if possible) *)
+  Lemma wp_Get_fail E get_i dst src pc_p pc_b pc_e pc_a w zsrc wdst :
+    decodeInstrW w = get_i →
+    is_Get get_i dst src →
+    isCorrectPC (WCap pc_p pc_b pc_e pc_a) →
+
+    {{{ ▷ PC ↦ᵣ WCap pc_p pc_b pc_e pc_a
+      ∗ ▷ pc_a ↦ₐ w
+      ∗ ▷ dst ↦ᵣ wdst
+      ∗ ▷ src ↦ᵣ WInt zsrc }}}
+      Instr Executable @ E
+      {{{ RET FailedV; True }}}.
+  Proof.
+    iIntros (Hdecode Hinstr Hvpc φ) "(>HPC & >Hpc_a & >Hsrc & >Hdst) Hφ".
+    iDestruct (map_of_regs_3 with "HPC Hsrc Hdst") as "[Hmap (%&%&%)]".
+    iApply (wp_Get with "[$Hmap Hpc_a]"); eauto; simplify_map_eq; eauto.
+      by erewrite regs_of_is_Get; eauto; rewrite !dom_insert; set_solver+.
+    iNext. iIntros (regs' retv) "(#Hspec & Hpc_a & Hmap)". iDestruct "Hspec" as %Hspec.
+    destruct Hspec as [* Hsucc |].
+    { (* Success (contradiction) *) simplify_map_eq. }
+    { (* Failure, done *) by iApply "Hφ". }
+  Qed.
+
+  (* TODO: move this to the rules_Lea.v file. *)
+  Lemma wp_Lea_fail_none Ep pc_p pc_b pc_e pc_a w r1 rv p b e a z :
+    decodeInstrW w = Lea r1 (inr rv) →
+    isCorrectPC (WCap pc_p pc_b pc_e pc_a) →
+    (a + z)%a = None ->
+
+     {{{ ▷ PC ↦ᵣ WCap pc_p pc_b pc_e pc_a
+           ∗ ▷ pc_a ↦ₐ w
+           ∗ ▷ r1 ↦ᵣ WCap p b e a
+           ∗ ▷ rv ↦ᵣ WInt z }}}
+       Instr Executable @ Ep
+     {{{ RET FailedV; True }}}.
+  Proof.
+    iIntros (Hdecode Hvpc Hz φ) "(>HPC & >Hpc_a & >Hsrc & >Hdst) Hφ".
+    iDestruct (map_of_regs_3 with "HPC Hsrc Hdst") as "[Hmap (%&%&%)]".
+    iApply (wp_lea with "[$Hmap Hpc_a]"); eauto; simplify_map_eq; eauto.
+      by rewrite !dom_insert; set_solver+.
+    iNext. iIntros (regs' retv) "(#Hspec & Hpc_a & Hmap)".
+    iDestruct "Hspec" as %Hspec.
+    destruct Hspec as [* Hsucc |].
+    { (* Success (contradiction) *) simplify_map_eq. }
+    { (* Failure, done *) by iApply "Hφ". }
+  Qed.
+
+  (* ------------------------------- *)
+
+
+  Definition reqperm_instrs r z :=
+    encodeInstrsW [
+        GetP r_t1 r
+        ; Sub r_t1 r_t1 z
+        ; Mov r_t2 PC
+        ; Lea r_t2 6
+        ; Jnz r_t2 r_t1
+        ; Mov r_t2 PC
+        ; Lea r_t2 4
+        ; Jmp r_t2
+        ; Fail
+        ; Mov r_t1 0
+        ; Mov r_t2 0].
+
+  Lemma reqperm_spec r perm w pc_p pc_b pc_e a_first w1 w2 φ :
+    ExecPCPerm pc_p →
+    SubBounds pc_b pc_e a_first (a_first ^+ length (reqperm_instrs r (encodePerm perm)))%a →
+
+      ▷ codefrag a_first (reqperm_instrs r (encodePerm perm))
+    ∗ ▷ PC ↦ᵣ WCap pc_p pc_b pc_e a_first
+    ∗ ▷ r ↦ᵣ w
+    ∗ ▷ r_t1 ↦ᵣ w1
+    ∗ ▷ r_t2 ↦ᵣ w2
+    ∗ ▷ (if isPermWord w perm then
+           ∃ b e a', ⌜w = WCap perm b e a'⌝ ∧
+           (PC ↦ᵣ WCap pc_p pc_b pc_e (a_first ^+ length (reqperm_instrs r (encodePerm perm)))%a
+            ∗ codefrag a_first (reqperm_instrs r (encodePerm perm)) ∗
+            r ↦ᵣ WCap perm b e a' ∗ r_t1 ↦ᵣ WInt 0%Z ∗ r_t2 ↦ᵣ WInt 0%Z
+            -∗ WP Seq (Instr Executable) {{ φ }})
+        else φ FailedV)
+    ⊢
+      WP Seq (Instr Executable) {{ φ }}.
+  Proof.
+    iIntros (Hvpc Hcont) "(>Hprog & >HPC & >Hr & >Hr_t1 & >Hr_t2 & Hφ)".
+    codefrag_facts "Hprog".
+    destruct w.
+    { (* if w is an integer, the getL will fail *)
+      iInstr_lookup "Hprog" as "Hi" "Hcont".
+      iInstr_get_rule "Hi" (fun rule => idtac rule).
+      wp_instr.
+      iApply (wp_Get_fail with "[$HPC $Hi $Hr_t1 $Hr]");iFrameCapSolve.
+      iNext. iIntros "_".
+      wp_pure.
+      iApply wp_value. done. }
+    (* if w is a capability, the getL will succeed *)
+    do 3 iInstr "Hprog".
+    destruct (isPermWord (WCap p b e a) perm) eqn:Hperm.
+    { iInstr "Hprog".
+      iInstr_lookup "Hprog" as "Hi" "Hcont".
+      iInstr_get_rule "Hi" (fun rule => idtac rule).
+      wp_instr.
+      assert (encodePerm p - encodePerm perm = 0)%Z as ->.
+      { inversion Hperm as [Hp]. apply bool_decide_eq_true_1 in Hp as ->. lia. }
+      iApply (wp_jnz_success_next with "[$HPC $Hi $Hr_t2 $Hr_t1]");iFrameCapSolve.
+      iNext. iIntros "(HPC & Hi & Hr_t2 & Hr_t1)". wp_pure.
+      iDestruct ("Hcont" with "Hi") as "Hprog".
+      iGo "Hprog".
+      rewrite -/(updatePcPerm (WCap pc_p pc_b pc_e (a_first ^+ 9)%a)).
+      rewrite updatePcPerm_cap_non_E;[|inv Hvpc;auto].
+      iGo "Hprog".
+      iDestruct "Hφ" as (b' e' a' Heq) "Hφ". inv Heq.
+      iApply "Hφ"; iFrame. }
+    { iGo "Hprog".
+      inversion Hperm as [Hp]. apply bool_decide_eq_false_1 in Hp. intros Hcontr; inversion Hcontr as [Heq].
+      apply Zminus_eq,encodePerm_inj in Heq. subst p. done.
+      rewrite -/(updatePcPerm (WCap pc_p pc_b pc_e (a_first ^+ 8)%a)).
+      rewrite updatePcPerm_cap_non_E;[|inv Hvpc;auto].
+      iGo "Hprog".
+      iApply wp_value. iFrame. }
+  Qed.
+
+  (* --------------------------------------- REQSIZE ----------------------------------- *)
+  (* This macro checks that the capability in r covers a memory range of size
+     (i.e. e-b) exactly equal to [minsize]. *)
+
+  Definition reqsize_exact_instrs r (exsize : Z) :=
+    encodeInstrsW
+      [ GetB r_t1 r ;
+      GetE r_t2 r;
+      Sub r_t1 r_t2 r_t1;
+      Sub r_t1 r_t1 exsize;
+      Mov r_t2 PC;
+      Lea r_t2 6;
+      Jnz r_t2 r_t1;
+      Mov r_t2 PC;
+      Lea r_t2 4;
+      Jmp r_t2;
+      Fail].
+
+  Lemma reqsize_spec r minsize pc_p pc_b pc_e a_first r_p r_b r_e r_a w1 w2 φ :
+    ExecPCPerm pc_p →
+    SubBounds pc_b pc_e a_first (a_first ^+ length (reqsize_exact_instrs r minsize))%a →
+
+      ▷ codefrag a_first (reqsize_exact_instrs r minsize)
+    ∗ ▷ PC ↦ᵣ WCap pc_p pc_b pc_e a_first
+    ∗ ▷ r ↦ᵣ WCap r_p r_b r_e r_a
+    ∗ ▷ r_t1 ↦ᵣ w1
+    ∗ ▷ r_t2 ↦ᵣ w2
+    ∗ ▷ (if (minsize =? (r_e - r_b)%a)%Z then
+           (∃ w1 w2,
+            codefrag a_first (reqsize_exact_instrs r minsize)
+            ∗ PC ↦ᵣ WCap pc_p pc_b pc_e (a_first ^+ length (reqsize_exact_instrs r minsize))%a
+            ∗ r ↦ᵣ WCap r_p r_b r_e r_a
+            ∗ r_t1 ↦ᵣ w1
+            ∗ r_t2 ↦ᵣ w2)
+           -∗ WP Seq (Instr Executable) {{ φ }}
+        else φ FailedV)
+    ⊢
+      WP Seq (Instr Executable) {{ φ }}.
+  Proof.
+    iIntros (Hvpc Hcont) "(>Hprog & >HPC & >Hr & >Hr_t1 & >Hr_t2 & Hφ)".
+    codefrag_facts "Hprog".
+    do 6 iInstr "Hprog".
+
+    destruct (minsize =? r_e - r_b)%Z eqn:Hsize.
+    { iInstr_lookup "Hprog" as "Hi" "Hcont".
+      iInstr_get_rule "Hi" (fun rule => idtac rule).
+      wp_instr.
+      assert (r_e - r_b - minsize = 0)%Z as ->.
+      { solve_addr. }
+      iApply (wp_jnz_success_next with "[$HPC $Hi $Hr_t2 $Hr_t1]");iFrameCapSolve.
+      iNext. iIntros "(HPC & Hi & Hr_t2 & Hr_t1)". wp_pure.
+      iDestruct ("Hcont" with "Hi") as "Hprog".
+      iGo "Hprog".
+      rewrite -/(updatePcPerm (WCap pc_p pc_b pc_e (a_first ^+ 11)%a)).
+      rewrite updatePcPerm_cap_non_E;[|by inv Hvpc].
+      iApply "Hφ". iExists _,_. iFrame. }
+    { iGo "Hprog". intros Hcontr. inv Hcontr. solve_addr.
+      rewrite -/(updatePcPerm (WCap pc_p pc_b pc_e (a_first ^+ 10)%a)).
+      rewrite updatePcPerm_cap_non_E;[|by inv Hvpc].
+      iGo "Hprog". iApply wp_value. iFrame. }
+  Qed.
+
   (* -------------------------------------- RCLEAR ----------------------------------- *)
   (* the following macro clears registers in r. a denotes the list of addresses
      containing the instructions for the clear: |a| = |r| *)
