theories/examples/dynamic_sealing_keys.v
@@ -1,0 +1,483 @@
+From iris.algebra Require Import frac auth list.
+From iris.proofmode Require Import tactics.
+Require Import Eqdep_dec List.
+From cap_machine Require Import macros_helpers addr_reg_sample macros_new.
+From cap_machine Require Import rules logrel contiguous.
+From cap_machine Require Import monotone keylist_new.
+From cap_machine Require Import solve_pure proofmode map_simpl.
+
+Section sealing.
+
+  Context {Σ:gFunctors} {memg:memG Σ} {regg:regG Σ}
+          {nainv: logrel_na_invs Σ}
+          `{MP: MachineParameters}
+          {mono : sealLLG Σ}.
+
+  (* Assume r_t1 contains a capability representing a sealed value.
+     First we must check that its permission is RWX (or the environment could derive
+     an O capability from the entrypoint to malloc), and that its range is 1
+     (to make sure it has the authority of a seal)
+     Get its b field, find the corresponding value in the linked list contained in r_env.
+     Result is returned in r_t1; clear r_env for security and return. *)
+  (* Arguments: r_t1
+     Return point: r_t0
+     Uses: r_env r_t4 (r_t2 rt_3 are used by findb) *)
+  Definition unseal_instrs :=
+    encodeInstrsW [ Mov r_t3 r_t1 ] ++
+    reqperm_instrs r_t3 (encodePerm RWX) ++
+    reqsize_exact_instrs r_t3 1 ++
+    encodeInstrsW [ GetB r_t1 r_t3
+                  ; Mov r_t4 (inr r_t0) (* Save return point *)
+                  ; Mov r_t0 (inr PC) (* Setup the return point for findb *)
+                  ; Lea r_t0 (inl (length findb_instr + 3)%Z)
+                  ] ++ (encodeInstrW (Load r_env r_env) :: findb_instr) ++
+    encodeInstrsW [ Mov r_env (inl 0%Z) (* Clearing *)
+                  ; Mov r_t0 (inr r_t4) (* Restore return capability *)
+                  ; Mov r_t4 (inl 0%Z) (* Clearing *)
+                  ; Jmp r_t0
+                  ].
+
+  Definition unseal_instrs_length := Eval cbn in length (unseal_instrs).
+
+  (* Assume r_t1 contains the word to seal.
+     Append it to the linked list contained in r_env.
+     Subseg the new capability to bottom range
+     clear r_env and return *)
+  (* Arguments: r_t1
+     Return point: r_t0
+     Uses: r_env r_t2 r_t7 (r_t3 r_t4 r_t5 r_t6 used by appendb) *)
+  Definition seal_instrs f_m :=
+    encodeInstrsW [ Mov r_t7 (inr r_t0) (* Save return point *)
+                  ; Mov r_t0 (inr PC) (* Setup the return point for findb *)
+                  ; Lea r_t0 (inl (length (appendb_instr f_m) + 2)%Z)
+                  ] ++ appendb_instr f_m ++
+    encodeInstrsW [ GetB r_t2 r_t1
+                  ; Add r_t3 r_t2 1
+                  ; Subseg r_t1 r_t2 r_t3
+                  ; Mov r_env (inl 0%Z) (* Clearing *)
+                  ; Mov r_t2 (inl 0%Z) (* Clearing *)
+                  ; Mov r_t3 (inl 0%Z) (* Clearing *)
+                  ; Mov r_t0 (inr r_t7) (* Restore return capability *)
+                  ; Mov r_t7 (inl 0%Z) (* Clearing *)
+                  ; Jmp r_t0
+                  ].
+
+  Definition seal_instrs_length := Eval cbn in length (seal_instrs 0%Z).
+
+  (* Create two closures for sealing and unsealing assuming that their code is preceding this one.
+     Specifically, we assume the memory layout is [unseal_instrs][seal_instrs][make_seal_preamble] *)
+  (* This works by:
+     1. Malloc an empty linked list, thus obtaining some capability c.
+     2. Create a closure with access to c, and containing the code unseal_instr.
+     3. Create a closure with access to c, and containing the code seal_instr.
+     4. Return closure for unsealing in r_t1 and sealing in r_t2. *)
+  (* Arguments: None
+     Return point: rt_0
+     Uses: r_t1 r_t2 r_t8 r_t9 r_t10 *)
+  Definition make_seal_preamble_instrs f_m :=
+    encodeInstrsW [ Mov r_t8 PC (* Copy PC into r_t8 *)
+                  ; Lea r_t8 (- (Z.of_nat seal_instrs_length))%Z (* Capability pointing to code for seal_instrs *)
+                  ]
+    ++ malloc_instrs f_m 1 ++ (* Malloc an empty list *)
+    encodeInstrsW [ Mov r_t9 r_t1 (* Keep a copy of the capability to the list *)
+                  ; Mov r_t2 r_t1 (* Prepare for creating closure, r_t2 must contain environment *)
+                  ; Mov r_t1 r_t8 (* Prepare for creating closure, r_t1 must contain code *)
+                  ]
+    ++ crtcls_instrs f_m ++ (* Create the closure for seal, result in r_t1 *)
+    encodeInstrsW [ Mov r_t10 r_t1 (* Closure for seal now in r_t10 *)
+                  ; Lea r_t8 (inl (- (Z.of_nat unseal_instrs_length))%Z) (* Capability pointing to code for seal_instrs *)
+                  ; Mov r_t1 r_t8 (* Prepare for creating closure for unseal, code *)
+                  ; Mov r_t2 r_t9 (* Prepare for creating closure for unseal, environment *)
+                  ]
+    ++ crtcls_instrs f_m ++ (* Create the closure for unseal, result in r_t1 *)
+    encodeInstrsW [ Mov r_t2 r_t10 (* Closure for seal now in r_t2 *)
+                  ; Mov r_t8 (inl 0%Z) (* Clearing registers *)
+                  ; Mov r_t9 (inl 0%Z)
+                  ; Mov r_t10 (inl 0%Z)
+                  ; Jmp r_t0 (* Return *)
+                  ].
+
+  Definition make_seal_preamble f_m ai :=
+    ([∗ list] a_i;w_i ∈ ai;(make_seal_preamble_instrs f_m), a_i ↦ₐ w_i)%I.
+
+  (* TODO: move this to the rules_Get.v file. small issue with the spec of failure: it does not actually
+     require/leave a trace on dst! It would be good if req_regs of a failing get does not include dst (if possible) *)
+  Lemma wp_Get_fail_same E get_i dst pc_p pc_b pc_e pc_a w zsrc :
+    decodeInstrW w = get_i →
+    is_Get get_i dst dst →
+    isCorrectPC (WCap pc_p pc_b pc_e pc_a) →
+
+    {{{ ▷ PC ↦ᵣ WCap pc_p pc_b pc_e pc_a
+      ∗ ▷ pc_a ↦ₐ w
+      ∗ ▷ dst ↦ᵣ WInt zsrc }}}
+      Instr Executable @ E
+      {{{ RET FailedV; True }}}.
+  Proof.
+    iIntros (Hdecode Hinstr Hvpc φ) "(>HPC & >Hpc_a & >Hsrc) Hφ".
+    iDestruct (map_of_regs_2 with "HPC Hsrc") as "[Hmap %]".
+    iApply (wp_Get with "[$Hmap Hpc_a]"); eauto; simplify_map_eq; eauto.
+      by erewrite regs_of_is_Get; eauto; rewrite !dom_insert; set_solver+.
+    iNext. iIntros (regs' retv) "(#Hspec & Hpc_a & Hmap)". iDestruct "Hspec" as %Hspec.
+    destruct Hspec as [* Hsucc |].
+    { (* Success (contradiction) *) simplify_map_eq. }
+    { (* Failure, done *) by iApply "Hφ". }
+  Qed.
+
+  Lemma unseal_spec pc_p pc_b pc_e (* PC *)
+        wret (* return cap *)
+        wsealed (* p b e a *) (* input cap *)
+        ll ll' (* linked list head and pointers *)
+        a_first (* special adresses *)
+        ι γ φ Ep (* invariant/gname names *)
+        Φ {Hpers : ∀ w, Persistent (Φ w)} (* this predicate is chosen by the client at creation *) :
+
+    (* PC assumptions *)
+    ExecPCPerm pc_p →
+
+    (* Program adresses assumptions *)
+    SubBounds pc_b pc_e a_first (a_first ^+ length unseal_instrs)%a →
+
+    (* linked list ptr element d *)
+    (ll + 1)%a = Some ll' →
+
+    up_close (B:=coPset) ι ⊆ Ep →
+
+    PC ↦ᵣ WCap pc_p pc_b pc_e a_first
+      ∗ r_t0 ↦ᵣ wret
+      ∗ r_env ↦ᵣ WCap RWX ll ll' ll
+      ∗ r_t1 ↦ᵣ (* WCap (p, b, e, a) *) wsealed
+      ∗ (∃ w, r_t2 ↦ᵣ w)
+      ∗ (∃ w, r_t3 ↦ᵣ w)
+      ∗ (∃ w, r_t4 ↦ᵣ w)
+      (* invariant for d *)
+      ∗ sealLL ι ll γ Φ
+      (* token which states all non atomic invariants are closed *)
+      ∗ na_own logrel_nais Ep
+      (* trusted code *)
+      ∗ codefrag a_first unseal_instrs
+      ∗ ▷ φ FailedV
+      ∗ ▷ (PC ↦ᵣ updatePcPerm wret
+          ∗ r_t0 ↦ᵣ wret
+          ∗ r_t2 ↦ᵣ WInt 0%Z
+          ∗ (∃ b b' a w pbvals, ⌜wsealed = WCap RWX b b' a ∧ (b + 1)%a = Some b' ∧ (b',w) ∈ pbvals⌝ ∗ prefLL γ pbvals ∗ r_t1 ↦ᵣ w ∗ r_env ↦ᵣ WInt 0%Z ∗ Φ w)
+          ∗ r_t3 ↦ᵣ WInt 0%Z
+          ∗ r_t4 ↦ᵣ WInt 0%Z
+          ∗ codefrag a_first unseal_instrs
+          ∗ na_own logrel_nais Ep
+          -∗ WP Seq (Instr Executable) {{ φ }})
+      -∗
+      WP Seq (Instr Executable) {{ φ }}.
+  Proof.
+    iIntros (Hvpc Hcont Hd Hnclose) "(HPC & Hr_t0 & Hr_env & Hr_t1 & Hr_t2 & Hr_t3 & Hr_t4 & #Hseal_inv & Hown & Hprog & Hφfailed & Hφ)".
+    iDestruct (big_sepL2_length with "Hprog") as %Hprog_length.
+    iDestruct "Hr_t2" as (w2) "Hr_t2".
+    iDestruct "Hr_t3" as (w3) "Hr_t3".
+    iDestruct "Hr_t4" as (w4) "Hr_t4".
+
+    focus_block_0 "Hprog" as "Hprog" "Hcont".
+    iInstr "Hprog".
+    unfocus_block "Hprog" "Hcont" as "Hprog".
+
+    focus_block 1 "Hprog" as mid Hmid "Hprog" "Hcont".
+    iApply reqperm_spec;iFrameCapSolve.
+    iNext. destruct (isPermWord wsealed RWX) eqn:Hperm;[|iFrame].
+    destruct wsealed as [z|p b e a];[inversion Hperm|].
+    apply bool_decide_eq_true_1 in Hperm as <-.
+    iExists _,_,_. iSplit;eauto. iIntros "(HPC & Hprog & Hr_t3 & Hr_t1 & Hr_t2)".
+    unfocus_block "Hprog" "Hcont" as "Hprog".
+
+    focus_block 2 "Hprog" as mid0 Hmid0 "Hprog" "Hcont".
+    iApply reqsize_spec;iFrameCapSolve.
+    iNext. destruct (1 =? e - b)%Z eqn:Hsize;cycle 1.
+    { iFrame. }
+    iIntros "HH". iDestruct "HH" as (w1 w0) "(Hprog & HPC & Hr_t3 & Hr_t1 & Hr_t2)".
+    unfocus_block "Hprog" "Hcont" as "Hprog".
+
+    codefrag_facts "Hprog". simpl in H, H0.
+    focus_block 3 "Hprog" as mid1 Hmid1 "Hprog" "Hcont".
+    iGo "Hprog". simpl in *. instantiate (1 := (mid1 ^+ 18)%a). solve_addr.
+    unfocus_block "Hprog" "Hcont" as "Hprog".
+
+    focus_block 4 "Hprog" as a_middle Ha_middle "Hprog" "Hcont".
+    iApply findb_spec; iFrameCapSolve; eauto.
+    iFrame "# ∗". iSplitL "Hr_t2"; eauto. iSplitL "Hr_t3"; eauto.
+    iNext. iIntros "(HPC & Hr_t0 & Hr_t2 & HisList & Hr_t3 & Hprog & Hown)".
+    iDestruct "HisList" as (b_a b' b'' w pbvals) "(%HX & Hpref & Hr_t1 & Hr_env & #HΦ)".
+    destruct HX as (HA & HA1 & HB & HC).
+    unfocus_block "Hprog" "Hcont" as "Hprog".
+    eapply z_to_addr_eq_inv in HA. subst b_a; auto.
+    assert (e = b')%Z as <-.
+    { solve_addr. }
+
+    rewrite (updatePcPerm_cap_non_E pc_p pc_b pc_e (mid1 ^+ 18)%a ltac:(destruct Hvpc; congruence)).
+    focus_block 5 "Hprog" as a_middle' Ha_middle' "Hprog" "Hcont".
+    iGo "Hprog".
+    unfocus_block "Hprog" "Hcont" as "Hprog".
+    iApply "Hφ"; iFrame "# ∗".
+    iExists _,_,_,_,_. iFrame "∗ #".
+    iPureIntro. eauto.
+  Qed.
+
+  Lemma seal_spec Φ (* client chosen seal predicate *)
+        pc_p pc_b pc_e (* PC *)
+        wret (* return cap *)
+        w (* input z *)
+        ll ll' pbvals (* linked list head and pointers *)
+        a_first (* special adresses *)
+        rmap (* register map *)
+        f_m b_m e_m (* malloc addrs *)
+        b_r e_r a_r a_r' (* environment table addrs *)
+        ι ι1 γ Ep φ (* invariant/gname names *)
+        {Hpers : ∀ w, Persistent (Φ w)} (* the client chosen predicate is persistent *) :
+
+    (* PC assumptions *)
+    ExecPCPerm pc_p →
+
+    (* Program adresses assumptions *)
+    SubBounds pc_b pc_e a_first (a_first ^+ length (seal_instrs f_m))%a →
+
+    (* linked list ptr element head *)
+    (ll + 1)%a = Some ll' →
+
+    dom (gset RegName) rmap = all_registers_s ∖ {[ PC; r_env; r_t0; r_t1 ]} →
+
+    (* environment table *)
+    withinBounds b_r e_r a_r' = true →
+    (a_r + f_m)%a = Some a_r' →
+
+    up_close (B:=coPset) ι ⊆ Ep →
+    up_close (B:=coPset) ι1 ⊆ Ep ∖ ↑ι →
+
+    PC ↦ᵣ WCap pc_p pc_b pc_e a_first
+       ∗ r_env ↦ᵣ WCap RWX ll ll' ll
+       ∗ r_t1 ↦ᵣ w
+       ∗ Φ w
+       ∗ r_t0 ↦ᵣ wret
+       ∗ ([∗ map] r↦w ∈ rmap, r ↦ᵣ w)
+       (* own token *)
+       ∗ na_own logrel_nais Ep
+       (* trusted code *)
+       ∗ codefrag a_first (seal_instrs f_m)
+       (* malloc *)
+       ∗ na_inv logrel_nais ι1 (malloc_inv b_m e_m)
+       ∗ pc_b ↦ₐ WCap RO b_r e_r a_r
+       ∗ a_r' ↦ₐ WCap E b_m e_m b_m
+       (* linked list invariants *)
+       ∗ sealLL ι ll γ Φ
+       ∗ prefLL γ pbvals
+       ∗ ▷ (PC ↦ᵣ updatePcPerm wret
+          ∗ r_env ↦ᵣ WInt 0%Z
+          ∗ r_t0 ↦ᵣ wret
+          ∗ pc_b ↦ₐ WCap RO b_r e_r a_r
+          ∗ a_r' ↦ₐ WCap E b_m e_m b_m
+          ∗ ([∗ map] r↦w ∈ <[r_t2:=WInt 0%Z]> (<[r_t3:=WInt 0%Z]> (<[r_t4:=WInt 0%Z]>
+                          (<[r_t5:=WInt 0%Z]> (<[r_t6:=WInt 0%Z]> (<[r_t7:=WInt 0%Z]> rmap))))), r ↦ᵣ w)
+          ∗ (∃ a a' pbvals', ⌜(a + 1)%a = Some a'⌝ ∗ prefLL γ (pbvals ++ pbvals' ++ [(a',w)]) ∗ r_t1 ↦ᵣ WCap RWX a a' a' ∗ a ↦ₐ WInt 0)
+          ∗ codefrag a_first (seal_instrs f_m)
+          ∗ na_own logrel_nais Ep
+          -∗ WP Seq (Instr Executable) {{ φ }})
+      -∗
+      WP Seq (Instr Executable) {{ λ v, φ v ∨ ⌜v = FailedV⌝ }}.
+  Proof.
+    iIntros (Hvpc Hcont Hhd Hdom Hbounds Hf_m Hnclose Hnclose') "(HPC & Hr_env & Hr_t1 & HΦw & Hr_t0 & Hregs & Hown & Hprog & #Hmalloc & Hpc_b & Ha_r' & #Hseal_inv & #Hpref & Hφ)".
+
+    codefrag_facts "Hprog".
+    focus_block_0 "Hprog" as "Hprog" "Hcont".
+    assert (is_Some (rmap !! r_t7)) as [w7 Hw7];[rewrite elem_of_gmap_dom Hdom; set_solver|].
+    iDestruct (big_sepM_delete _ _ r_t7 with "Hregs") as "[Hr_t7 Hregs]";[apply Hw7|].
+    iGo "Hprog".
+    unfocus_block "Hprog" "Hcont" as "Hprog".
+    iDestruct (big_sepM_insert _ _ r_t7 with "[$Hregs $Hr_t7]") as "Hregs"; [apply lookup_delete|].
+    rewrite insert_delete.
+
+    focus_block 1 "Hprog" as a_middle Ha_middle "Hprog" "Hcont".
+    iApply appendb_spec; try iFrame "∗ #"; auto. rewrite dom_insert_L Hdom. set_solver.
+    iFrame. iNext. iIntros "(HPC & Hr_env & Hr_t0 & Hpc_b & Ha_r' & Hregs & HisList & Hprog & Hown)".
+    unfocus_block "Hprog" "Hcont" as "Hprog".
+
+    rewrite (updatePcPerm_cap_non_E pc_p pc_b pc_e (a_first ^+ 54)%a ltac:(destruct Hvpc; congruence)).
+    focus_block 2 "Hprog" as a_middle' Ha_middle' "Hprog" "Hcont".
+    iDestruct (big_sepM_delete _ _ r_t7 with "Hregs") as "[Hr_t7 Hregs]";[simplify_map_eq; auto|].
+    iDestruct (big_sepM_delete _ _ r_t2 with "Hregs") as "[Hr_t2 Hregs]";[simplify_map_eq; auto|].
+    iDestruct (big_sepM_delete _ _ r_t3 with "Hregs") as "[Hr_t3 Hregs]";[simplify_map_eq; auto|].
+    map_simpl "Hregs".
+    iDestruct "HisList" as (a a' a'' pbvals') "(%HA & #Hpref' & Hr_t1 & Ha)".
+    destruct HA as (HA & HB).
+    iGo "Hprog". instantiate (1:=a'). solve_addr. solve_addr.
+    iGo "Hprog". (* rewrite decode_encode_perm_inv. reflexivity. *)
+    (* iGo "Hprog". rewrite decode_encode_perm_inv. auto. solve_addr. *)
+    (* iGo "Hprog". *)
+    unfocus_block "Hprog" "Hcont" as "Hprog".
+    iApply "Hφ"; iFrame "∗ #".
+    iSplitR "Hr_t1 Ha ".
+    - iDestruct (big_sepM_insert _ _ r_t3 with "[$Hregs $Hr_t3]") as "Hregs"; [apply lookup_delete|].
+      map_simpl "Hregs".
+      iDestruct (big_sepM_insert _ _ r_t2 with "[$Hregs $Hr_t2]") as "Hregs"; [simplify_map_eq;auto|].
+      map_simpl "Hregs".
+      iDestruct (big_sepM_insert _ _ r_t7 with "[$Hregs $Hr_t7]") as "Hregs"; [simplify_map_eq;auto|].
+      map_simpl "Hregs".
+      repeat rewrite -(insert_commute _ _ r_t7)//.
+    - iExists _, _, _. iFrame. iSplit;eauto.
+  Qed.
+
+  Lemma sealLL_alloc ι ll Ep Φ {Hpers : ∀ w, Persistent (Φ w)} :
+    ll ↦ₐ WInt 0%Z -∗
+    |={Ep}=> ∃ γ, sealLL ι ll γ Φ.
+  Proof.
+    iIntros "Hll".
+    iMod (own_alloc (● principal prefR [])) as (γ) "Hown".
+    { eapply auth_auth_valid. repeat red. apply I. }
+    iMod (na_inv_alloc logrel_nais _ ι (∃ hd : Word, ll ↦ₐ hd ∗ (∃ awvals : list (Addr * Word), isList hd awvals ∗ Exact γ awvals ∗ [∗ list] aw ∈ awvals, Φ aw.2)) with "[Hll Hown]")%I as "Hinv".
+    { iNext. iExists (WInt 0%Z). iFrame.
+      iExists []. iFrame. iSplit;done. }
+    iExists γ. auto.
+  Qed.
+
+  Lemma make_seal_spec pc_p pc_b pc_e (* PC *)
+        wret (* return cap *)
+        a_first (* special adresses *)
+        rmap (* register map *)
+        f_m b_m e_m (* malloc addrs *)
+        b_r e_r a_r a_r' (* environment table addrs *)
+        ι ι1 Ep φ (* invariant/gname names *)
+        Φ {Hpers: ∀ w, Persistent (Φ w)} (* The spec for make seal works for any seal predicate Φ
+             that the client must choose upon creation *) :
+
+    (* PC assumptions *)
+    ExecPCPerm pc_p →
+
+    (* Program adresses assumptions *)
+    SubBounds pc_b pc_e a_first (a_first ^+ (length (unseal_instrs) + length (seal_instrs f_m) + length (make_seal_preamble_instrs f_m)))%a →
+
+    dom (gset RegName) rmap = all_registers_s ∖ {[ PC; r_t0]} →
+
+    (* environment table *)
+    withinBounds b_r e_r a_r' = true →
+    (a_r + f_m)%a = Some a_r' →
+
+    up_close (B:=coPset) ι1 ⊆ Ep →
+
+    PC ↦ᵣ WCap pc_p pc_b pc_e (a_first ^+ (length (unseal_instrs) + length (seal_instrs f_m)))%a
+       ∗ r_t0 ↦ᵣ wret
+       ∗ ([∗ map] r↦w ∈ rmap, r ↦ᵣ w)
+       (* own token *)
+       ∗ na_own logrel_nais Ep
+       (* trusted code *)
+       ∗ codefrag a_first (unseal_instrs ++ seal_instrs f_m ++ make_seal_preamble_instrs f_m)
+       (* malloc *)
+       ∗ na_inv logrel_nais ι1 (malloc_inv b_m e_m)
+       ∗ pc_b ↦ₐ WCap RO b_r e_r a_r
+       ∗ a_r' ↦ₐ WCap E b_m e_m b_m
+       ∗ ▷ (PC ↦ᵣ updatePcPerm wret
+          ∗ r_t0 ↦ᵣ wret
+          ∗ pc_b ↦ₐ WCap RO b_r e_r a_r
+          ∗ a_r' ↦ₐ WCap E b_m e_m b_m
+          ∗ (∃ b1 e1 b2 e2 ll ll', let wvar := WCap RWX ll ll' ll in
+                                   let wcode1 := WCap pc_p pc_b pc_e a_first in
+                                   let wcode2 := WCap pc_p pc_b pc_e (a_first ^+ length (unseal_instrs))%a in
+                                   r_t1 ↦ᵣ WCap E b1 e1 b1 ∗ r_t2 ↦ᵣ WCap E b2 e2 b2
+                                   ∗ ⌜(b1 + 8)%a = Some e1⌝ ∗ ⌜(b2 + 8)%a = Some e2⌝
+                                   ∗ [[b1,e1]]↦ₐ[[activation_instrs wcode1 wvar]]
+                                   ∗ [[b2,e2]]↦ₐ[[activation_instrs wcode2 wvar]]
+                                   (* linked list invariants *)
+                                   ∗ ⌜(ll + 1)%a = Some ll'⌝
+                                   ∗ ∃ γ, sealLL ι ll γ Φ)
+          ∗ ([∗ map] r↦w ∈ (<[r_t3:=WInt 0%Z]> (<[r_t4:=WInt 0%Z]> (<[r_t5:=WInt 0%Z]> (<[r_t6:=WInt 0%Z]> (<[r_t7:=WInt 0%Z]> (<[r_t8:=WInt 0%Z]> (<[r_t9:=WInt 0%Z]> (<[r_t10:=WInt 0%Z]> (delete r_t1 (delete r_t2 rmap)))))))))), r ↦ᵣ w)
+          ∗ codefrag a_first (unseal_instrs ++ seal_instrs f_m ++ make_seal_preamble_instrs f_m)
+          ∗ na_own logrel_nais Ep
+          -∗ WP Seq (Instr Executable) {{ φ }})
+      -∗
+      WP Seq (Instr Executable) {{ λ v, φ v ∨ ⌜v = FailedV⌝ }}.
+  Proof.
+    iIntros (Hvpc Hcont Hdom Hbounds Hf_m Hnclose') "(HPC & Hr_t0 & Hregs & Hown & Hprog & #Hmalloc & Hpc_b & Ha_r' & Hφ)".
+
+    focus_block 2 "Hprog" as a_middle Ha_middle "Hprog" "Hcont".
+    assert (is_Some (rmap !! r_t8)) as [w8 Hw8];[rewrite elem_of_gmap_dom Hdom; set_solver|].
+    iDestruct (big_sepM_delete _ _ r_t8 with "Hregs") as "[Hr_t8 Hregs]";[apply Hw8|].
+    iGo "Hprog".
+    { rewrite /seal_instrs_length. instantiate (1 := (a_first ^+ length (unseal_instrs))%a).
+      solve_addr. }
+    unfocus_block "Hprog" "Hcont" as "Hprog".
+
+    iDestruct (big_sepM_insert _ _ r_t8 with "[$Hregs $Hr_t8]") as "Hregs"; [apply lookup_delete|].
+    rewrite insert_delete.
+
+    rewrite /make_seal_preamble_instrs.
+    focus_block 3 "Hprog" as a_middle1 Ha_middle1 "Hprog" "Hcont".
+    iApply malloc_spec_alt; iFrameCapSolve. 4: iFrame "# ∗".
+    set_solver. auto. lia.
+    iSplitL "". iNext. auto.
+    iSplitL "". iNext. iRight. auto.
+    iNext. iIntros "(HPC & Hprog & Hpc_b & Ha_r' & Hll & Hr_t0 & Hown & Hregs)".
+    iDestruct "Hll" as (ll ll') "(%Heqb & Hr_t1 & Hll)".
+    unfocus_block "Hprog" "Hcont" as "Hprog".
+
+    focus_block 4 "Hprog" as a_middle2 Ha_middle2 "Hprog" "Hcont".
+    iDestruct (big_sepM_delete _ _ r_t8 with "Hregs") as "[Hr_t8 Hregs]";[simplify_map_eq; auto|].
+    iDestruct (big_sepM_delete _ _ r_t2 with "Hregs") as "[Hr_t2 Hregs]";[simplify_map_eq; auto|].
+    assert (is_Some (rmap !! r_t9)) as [w9 Hw9];[rewrite elem_of_gmap_dom Hdom; set_solver|].
+    iDestruct (big_sepM_delete _ _ r_t9 with "Hregs") as "[Hr_t9 Hregs]";[simplify_map_eq; auto|].
+    map_simpl "Hregs".
+    iGo "Hprog".
+    unfocus_block "Hprog" "Hcont" as "Hprog".
+
+    iDestruct (big_sepM_insert _ _ r_t9 with "[$Hregs $Hr_t9]") as "Hregs"; [apply lookup_delete|].
+    iDestruct (big_sepM_insert _ _ r_t8 with "[$Hregs $Hr_t8]") as "Hregs"; [simplify_map_eq; auto|].
+    (* TODO debug why map_simpl "Hregs" loops here ?? *)
+    rewrite insert_delete. rewrite (delete_commute _ _ r_t8)//.
+    rewrite -(delete_insert_ne _ r_t8); auto. rewrite insert_delete.
+
+    focus_block 5 "Hprog" as a_middle3 Ha_middle3 "Hprog" "Hcont".
+    iApply crtcls_spec_alt; iFrameCapSolve. 3: iFrame "# ∗".
+    set_solver+ Hdom. auto.
+    iSplitL ""; eauto. iSplitL ""; eauto.
+    iNext. iIntros "(HPC & Hprog & Hpc_b & Ha_r' & Hseal)".
+    iDestruct "Hseal" as (b1 e1) "(Hb1eq & Hr_t1 & Hseal & Hr_t0 & Hr_t2 & Hown & Hregs)".
+    unfocus_block "Hprog" "Hcont" as "Hprog".
+
+    focus_block 6 "Hprog" as a_middle4 Ha_middle4 "Hprog" "Hcont".
+    iDestruct (big_sepM_delete _ _ r_t8 with "Hregs") as "[Hr_t8 Hregs]";[simplify_map_eq; auto|].
+    iDestruct (big_sepM_delete _ _ r_t9 with "Hregs") as "[Hr_t9 Hregs]";[simplify_map_eq; auto|].
+    assert (is_Some (rmap !! r_t10)) as [w10 Hw10];[rewrite elem_of_gmap_dom Hdom; set_solver|].
+    iDestruct (big_sepM_delete _ _ r_t10 with "Hregs") as "[Hr_t10 Hregs]";[simplify_map_eq; auto|].
+    map_simpl "Hregs".
+    iGo "Hprog". instantiate (1 := a_first). rewrite /unseal_instrs_length. solve_addr.
+    iGo "Hprog".
+    unfocus_block "Hprog" "Hcont" as "Hprog".
+
+    focus_block 7 "Hprog" as a_middle5 Ha_middle5 "Hprog" "Hcont".
+    iDestruct (big_sepM_insert _ _ r_t9 with "[$Hregs $Hr_t9]") as "Hregs"; [simplify_map_eq; auto|].
+    iDestruct (big_sepM_insert _ _ r_t8 with "[$Hregs $Hr_t8]") as "Hregs"; [simplify_map_eq; auto|].
+    iDestruct (big_sepM_insert _ _ r_t10 with "[$Hregs $Hr_t10]") as "Hregs"; [simplify_map_eq; auto|].
+    map_simpl "Hregs".
+    iApply crtcls_spec; iFrameCapSolve. 3: iFrame "# ∗".
+    set_solver+ Hdom. auto.
+    iNext. iIntros "(HPC & Hprog & Hpc_b & Ha_r' & Hunseal)".
+    iDestruct "Hunseal" as (b2 e2) "(Hb2eq & Hr_t1 & Hunseal & Hr_t0 & Hr_t2 & Hown & Hregs)".
+    map_simpl "Hregs".
+    unfocus_block "Hprog" "Hcont" as "Hprog".
+
+    focus_block 8 "Hprog" as a_middle6 Ha_middle6 "Hprog" "Hcont".
+    iDestruct (big_sepM_delete _ _ r_t8 with "Hregs") as "[Hr_t8 Hregs]";[simplify_map_eq; auto|].
+    iDestruct (big_sepM_delete _ _ r_t9 with "Hregs") as "[Hr_t9 Hregs]";[simplify_map_eq; auto|].
+    iDestruct (big_sepM_delete _ _ r_t10 with "Hregs") as "[Hr_t10 Hregs]";[simplify_map_eq; auto|].
+    iGo "Hprog".
+    unfocus_block "Hprog" "Hcont" as "Hprog".
+
+    iMod (sealLL_alloc with "[Hll]") as (γ) "Hsealinv".
+    { rewrite /region_mapsto. rewrite region_addrs_single; auto.
+      rewrite /region_addrs_zeroes. rewrite (proj2 (proj1 (incr_addr_region_size_iff ll ll' 1) ltac:(auto))).
+      simpl replicate. iDestruct "Hll" as "(Hll & _)". iFrame. }
+    iDestruct (big_sepM_insert _ _ r_t9 with "[$Hregs $Hr_t9]") as "Hregs"; [simplify_map_eq; auto|].
+    iDestruct (big_sepM_insert _ _ r_t8 with "[$Hregs $Hr_t8]") as "Hregs"; [simplify_map_eq; auto|].
+    iDestruct (big_sepM_insert _ _ r_t10 with "[$Hregs $Hr_t10]") as "Hregs"; [simplify_map_eq; auto|].
+    map_simpl "Hregs".
+    iApply "Hφ"; iFrame "∗ #".
+    iSplitR "Hregs".
+    { iExists b2, e2, b1, e1, ll, ll'. iFrame "∗".
+      iFrame "%". iExists γ. iFrame. }
+    { rewrite delete_commute //.
+      rewrite !(insert_commute _ r_t3) // !(insert_commute _ r_t4) // !(insert_commute _ r_t5) // !(insert_commute _ r_t6) // !(insert_commute _ r_t7) // !(insert_commute _ r_t8) // !(insert_commute _ r_t9) // !(insert_commute _ r_t10) //. }
+  Qed.
+
+End sealing.
